partial progress on zHEAP_DEREF
got stuck because x64_payload_def is wrong (and possibly other
problems...)

x86-64/x64_heapScript.sml
@@ -362,6 +362,12 @@ val isRefPtr_def = Define `
 
 val getRefPtr_def = Define `(getRefPtr (RefPtr x) = x) /\ (getRefPtr _ = ARB)`;
 
+val isValueArray_def = Define`
+  (isValueArray (ValueArray _) = T) /\
+  (isValueArray _ = F)`
+val getValueArray_def = Define`
+  (getValueArray (ValueArray v) = v)`
+
 val isCodePtr_def = Define `
   (isCodePtr (CodePtr _) = T) /\ (isCodePtr _ = F)`;
 
@@ -3729,7 +3735,7 @@ gg goal
 
 (* el *)
 
-val el_lemma =
+val el_lemma1 =
   abs_ml_inv_stack_permute
   |> Q.SPECL [`[(x1,r1);(x2,r2);(x3,r3)]`,`[(x1,r1);(x2,r2)]`]
   |> SIMP_RULE std_ss [MAP,APPEND,SUBSET_DEF,MEM] |> GEN_ALL
@@ -3824,7 +3830,7 @@ gg goal
       \\ FULL_SIMP_TAC std_ss [ADD1,AC ADD_COMM ADD_ASSOC]
       \\ FULL_SIMP_TAC std_ss [GSYM APPEND_ASSOC,APPEND]
       \\ REPEAT STRIP_TAC
-      \\ MATCH_MP_TAC el_lemma
+      \\ MATCH_MP_TAC el_lemma1
       \\ METIS_TAC [])
     \\ FULL_SIMP_TAC std_ss [LENGTH,LENGTH_APPEND]
     \\ FULL_SIMP_TAC std_ss [ADD1,AC ADD_COMM ADD_ASSOC]
@@ -8565,56 +8571,108 @@ gg goal
 
 (*
 val zHEAP_DEREF = let
-  val th = compose_specs ["mov r0,[r0+9]"]
+  val th = compose_specs ["mov r0,[r1+2*r0+9]"]
   val pc = get_pc th
   val target = ``~zS * zPC p * zVALS cs vals *
-      cond (heap_inv (cs,x1,x2,x3,x4,refs,stack,s,NONE) vals /\ isRefPtr x1)``
+      cond (heap_inv (cs,x1,x2,x3,x4,refs,stack,s,NONE) vals /\
+            isRefPtr x2 /\ isNumber x1 /\ 0 <= getNumber x1 /\
+            isValueArray (refs ' (getRefPtr x2)) /\
+            getNumber x1 < & LENGTH (getValueArray (refs ' (getRefPtr x2))))``
   val (th,goal) = expand_pre th target
   val lemma = prove(goal, SIMP_TAC (std_ss++star_ss) [zVALS_def,SEP_IMP_REFL])
   val th = MP th lemma |> DISCH_ALL |> DISCH T
                        |> PURE_REWRITE_RULE [AND_IMP_INTRO]
   val th = MATCH_MP SPEC_WEAKEN_LEMMA th
-  val th = th |> Q.SPEC `zHEAP (cs,refs ' (getRefPtr x1),x2,x3,x4,
+  val th = th |> Q.SPEC `zHEAP (cs,EL (Num (getNumber x1)) (getValueArray (refs ' (getRefPtr x2))),x2,x3,x4,
                                 refs,stack,s,NONE) * ~zS * ^pc`
   val goal = th |> concl |> dest_imp |> fst
+  (* gg goal *)
   val lemma = prove(goal,
     SIMP_TAC std_ss [LET_DEF,SEP_CLAUSES]
     \\ SIMP_TAC std_ss [zHEAP_def,SEP_IMP_def,SEP_CLAUSES,SEP_EXISTS_THM]
     \\ SIMP_TAC std_ss [Once heap_inv_def] \\ STRIP_TAC
-    \\ Cases_on `x1` \\ FULL_SIMP_TAC std_ss [isRefPtr_def,APPEND]
+    \\ Cases_on `x2` \\ FULL_SIMP_TAC std_ss [isRefPtr_def,APPEND,getRefPtr_def]
+    \\ Cases_on `x1` \\ FULL_SIMP_TAC std_ss [isNumber_def,APPEND,getNumber_def]
+    \\ Cases_on `refs ' n` \\ FULL_SIMP_TAC std_ss [isValueArray_def,getValueArray_def]
+    \\ Cases_on `l = []` \\ FULL_SIMP_TAC std_ss []
+    THEN1 (FULL_SIMP_TAC std_ss [LENGTH] \\ `F` by intLib.COOPER_TAC)
+    \\ `Num i < LENGTH l` by intLib.COOPER_TAC
+    \\ `abs_ml_inv (RefPtr n::Number i::x3::x4::stack) refs
+         (r2::r1::r3::r4::roots,heap,a,sp) cs.heap_limit` by
+       (MATCH_MP_TAC el_lemma2 \\ fs [] \\ REPEAT STRIP_TAC \\ fs [])
     \\ IMP_RES_TAC deref_thm
-    \\ `abs_ml_inv (refs ' n::x2::x3::x4::stack) refs
-         (y::r2::r3::r4::roots,heap,a,sp) cs.heap_limit` by ALL_TAC
-    THEN1 (MATCH_MP_TAC (cons_lemma |> GEN_ALL) \\ METIS_TAC [])
-    \\ POP_ASSUM MP_TAC \\ POP_ASSUM (K ALL_TAC) \\ STRIP_TAC
-    \\ Q.PAT_ASSUM `heap_el r 0 heap = (y,T)` (ASSUME_TAC o GSYM)
+    \\ POP_ASSUM (Q.SPEC_THEN`Num i`STRIP_ASSUME_TAC)
+    \\ `Num i < LENGTH ts` by fs[]
+    \\ POP_ASSUM (fn th => POP_ASSUM (STRIP_ASSUME_TAC o C MATCH_MP th))
+    \\ Q.PAT_ASSUM `heap_el r (Num i) heap = (y,T)` (ASSUME_TAC o GSYM)
     \\ Q.PAT_ASSUM `r1::r2::r3::r4::roots = r::roots2` (ASSUME_TAC o GSYM)
-    \\ FULL_SIMP_TAC std_ss [heap_el_def,CONS_11]
-    \\ `?f. (r1 = Pointer (f ' n)) /\ bc_ref_inv n refs (f,heap)` by ALL_TAC THEN1
+    \\ FULL_SIMP_TAC std_ss [CONS_11]
+    \\ `?f. (r2 = Pointer (f ' n)) /\ bc_ref_inv n refs (f,heap)` by ALL_TAC THEN1
       (FULL_SIMP_TAC std_ss [abs_ml_inv_def,bc_stack_ref_inv_def,LIST_REL_def,
         bc_value_inv_def] \\ Q.LIST_EXISTS_TAC [`f`]
       \\ ASM_SIMP_TAC std_ss []
-      \\ `reachable_refs (RefPtr n::x2::x3::x4::stack) refs n` by ALL_TAC THEN1
+      \\ `reachable_refs (Number i::RefPtr n::x3::x4::stack) refs n` by ALL_TAC THEN1
        (FULL_SIMP_TAC std_ss [reachable_refs_def,MEM]
         \\ Q.LIST_EXISTS_TAC [`RefPtr n`,`n`]
         \\ FULL_SIMP_TAC std_ss [get_refs_def,MEM,RTC_REFL])
-      \\ RES_TAC)
-    \\ FULL_SIMP_TAC std_ss [heap_el_def,bc_ref_inv_def,RefBlock_def]
-    \\ FULL_SIMP_TAC (srw_ss()) []
+      \\ RES_TAC \\ fs[])
+    \\ rpt(qpat_assum`T`kall_tac)
+    \\ rpt BasicProvers.VAR_EQ_TAC
+    \\ fs[bc_ref_inv_def,heap_el_def,FLOOKUP_DEF]
+    \\ Cases_on`n IN FDOM f` \\ fs[]
+    \\ Cases_on`n IN FDOM refs` \\ fs[]
+    \\ Cases_on`refs ' n` \\ fs[RefBlock_def] \\ fs[]
+    \\ Cases_on`Num i < LENGTH zs` \\ fs[]
+    \\ rpt BasicProvers.VAR_EQ_TAC
+    \\ rpt(qpat_assum`T`kall_tac)
     \\ IMP_RES_TAC heap_lookup_SPLIT
     \\ FULL_SIMP_TAC (std_ss++sep_cond_ss) [x64_heap_APPEND,x64_heap_def,x64_el_def,
          x64_payload_def,SEP_CLAUSES,cond_STAR,MAP,LET_DEF,LENGTH,one_list_def,
          x64_addr_def,WORD_MUL_LSL]
-    \\ SIMP_TAC std_ss [CONJ_ASSOC] \\ STRIP_TAC THEN1
-     (FULL_SIMP_TAC std_ss [word_arith_lemma3,word_mul_n2w,
-        AC MULT_COMM MULT_ASSOC] \\ SEP_R_TAC
-      \\ FULL_SIMP_TAC std_ss [GSYM word_mul_n2w]
-      \\ ONCE_REWRITE_TAC [WORD_AND_COMM]
-      \\ SIMP_TAC std_ss [blast_lemma] \\ FULL_SIMP_TAC std_ss [heap_vars_ok_def])
-    \\ FULL_SIMP_TAC std_ss [word_arith_lemma3,word_mul_n2w,
-         AC MULT_COMM MULT_ASSOC] \\ SEP_R_TAC
+    \\ SIMP_TAC std_ss [WORD_ADD_ASSOC,WORD_SUB_ADD]
+    \\ `r1 = Data (2w * n2w (Num i))` by ALL_TAC THEN1
+     (`small_int i /\ ~(i < 0)` by ALL_TAC THEN1
+        (FULL_SIMP_TAC std_ss [small_int_def] \\ intLib.COOPER_TAC)
+      \\ FULL_SIMP_TAC std_ss [abs_ml_inv_def,bc_stack_ref_inv_def,LIST_REL_def,
+            bc_value_inv_def])
+    \\ FULL_SIMP_TAC (srw_ss()) [x64_addr_def,WORD_MUL_LSL,w2w_def,word_mul_n2w]
+    \\ `(2 * Num i) < 9223372036854775808` by DECIDE_TAC
+    \\ FULL_SIMP_TAC std_ss [MULT_ASSOC]
+    \\ IMP_RES_TAC LESS_LENGTH \\ NTAC 2 (POP_ASSUM (K ALL_TAC))
+    \\ Q.MATCH_ASSUM_RENAME_TAC `xs = zs1 ++ z::zs2` []
+    \\ FULL_SIMP_TAC std_ss [MAP,MAP_APPEND,one_list_APPEND,one_list_def,
+         LENGTH_MAP]
+    \\ FULL_SIMP_TAC std_ss [GSYM word_mul_n2w,AC WORD_ADD_COMM WORD_ADD_ASSOC,
+         AC WORD_MULT_ASSOC WORD_MULT_COMM]
+    \\ SEP_R_TAC \\ STRIP_TAC THEN1
+     (SIMP_TAC std_ss [] \\ ONCE_REWRITE_TAC [WORD_AND_COMM]
+      \\ SIMP_TAC std_ss [WORD_ADD_ASSOC,blast_align_lemma]
+      \\ FULL_SIMP_TAC std_ss [heap_vars_ok_def])
     \\ REPEAT STRIP_TAC
-    \\ Q.EXISTS_TAC `vals with <| reg0 := x64_addr vs.current_heap y' |>`
+    \\ Q.EXISTS_TAC `vals with <| reg0 := x64_addr vs.current_heap z |>`
+    \\ Tactical.REVERSE STRIP_TAC THEN1
+     (POP_ASSUM MP_TAC \\ FULL_SIMP_TAC (srw_ss()) [zVALS_def]
+      \\ FULL_SIMP_TAC std_ss [GSYM APPEND_ASSOC,APPEND]
+      \\ FULL_SIMP_TAC (srw_ss()++star_ss) [])
+    \\ FULL_SIMP_TAC (srw_ss()) [heap_inv_def]
+    \\ Q.LIST_EXISTS_TAC [`vs`,`z`,`r2`,`r3`,`r4`,`roots`,
+                          `heap`,`a`,`sp`]
+    \\ FULL_SIMP_TAC (std_ss++star_ss) [word_mul_n2w] \\ POP_ASSUM (K ALL_TAC)
+    \\ FULL_SIMP_TAC (std_ss++sep_cond_ss) [x64_heap_APPEND,x64_heap_def,x64_el_def,
+         x64_payload_def,SEP_CLAUSES,cond_STAR,MAP,LET_DEF,LENGTH,one_list_def,
+         x64_addr_def,WORD_MUL_LSL,BlockRep_def]
+    \\ STRIP_TAC THEN1
+     (Q.PAT_ASSUM `abs_ml_inv xx yy zz tt` MP_TAC
+      \\ FULL_SIMP_TAC std_ss [LIST_REL_EL_EQN]
+      \\ `EL (Num i) (zs1 ++ z::zs2) = z` by METIS_TAC [EL_LENGTH]
+      \\ first_x_assum(qspec_then`Num i`mp_tac)
+      \\ simp[]
+      \\ FULL_SIMP_TAC std_ss [ADD1,AC ADD_COMM ADD_ASSOC]
+      \\ FULL_SIMP_TAC std_ss [GSYM APPEND_ASSOC,APPEND]
+      \\ REPEAT STRIP_TAC
+      \\ MATCH_MP_TAC el_lemma1
+      \\ METIS_TAC [])
+
     \\ FULL_SIMP_TAC std_ss [zVALS_def]
     \\ FULL_SIMP_TAC std_ss [GSYM APPEND_ASSOC,APPEND]
     \\ FULL_SIMP_TAC (srw_ss()++star_ss) []
